[SI] read proven (modulo model lemmas).

aneris/examples/snapshot_isolation/proof/resources/proxy_resources.v
@@ -24,31 +24,7 @@ Import gen_heap_light.
 
 Inductive proxy_state : Type :=
 | PSCanStart
-| PSActive of (gmap Key (list write_event)).
-
-Definition hist_to_we (h : list write_event) := last h.
-
-Definition to_hist (h : list write_event) : list val := (λ e, e.(we_val)) <$> h.
-
-Lemma to_hist_prefix_mono hw hw' :
-  hw `prefix_of` hw' →  to_hist hw `prefix_of` to_hist hw'.
-Proof.
-  intros Hp.
-  generalize dependent hw'.
-  induction hw as [|x l]; intros hw' Hp.
-  - by apply prefix_nil.
-  - destruct hw' as [|x' l'].
-    -- by apply prefix_nil_not in Hp.
-    -- simplify_eq /=.
-       assert (x = x') as -> by by apply prefix_cons_inv_1 in Hp.
-       apply prefix_cons.
-       apply IHl.
-       by apply prefix_cons_inv_2 in Hp.
-Qed.
-
-  
-Definition socket_address_to_str (sa : socket_address) : string :=
-    match sa with SocketAddressInet ip p => ip +:+ (string_of_pos p) end.
+| PSActive of global_mem.
 
 Section Proxy.
   Context `{!anerisG Mdl Σ, !User_params, !IDBG Σ, !MTS_resources }.
@@ -301,7 +277,6 @@ Section Proxy.
                   by apply (H_coh_8 k'). 
                 }
   Qed.
-
 
   Definition cacheM_from_Msnap (M : gmap Key (list write_event))
     : gmap Key (option val * bool) :=
